start proving things about our top-level procedures, starting with smc_handler

verified/main.dfy
@@ -12,7 +12,7 @@ method printSMCHandlerReturn()
     printInsFixed("MOVS", "pc, lr");
 }
 
-method Main()
+method printAll()
 {
     var n := 0;
     var monitor_vectbl := emptyVecTbl().(svc_smc := Just("smc"));
@@ -42,4 +42,47 @@ method Main()
 
     printBss(KomGlobalDecls());
     printFooter();
+}
+
+// this is what we assume about the initial state on entry to the SMC handler
+predicate InitialState(s:state)
+{
+    reveal_ValidRegState();
+
+    SaneConstants()
+        && ValidState(s) && s.ok
+        && mode_of_state(s) == Monitor
+        && s.conf.scr.ns == NotSecure
+        && s.regs[SP(Monitor)] == StackBase()
+        && SaneMem(s.m)
+}
+
+method Main()
+{
+    var smc_handler := sp_code_smc_handler();
+    var svc_handler := sp_code_svc_handler();
+    var abt_handler := sp_code_abort_handler();
+
+    // prove that the final state for an SMC call is valid
+    forall s1:state, p1:PageDb, s2:state
+        | InitialState(s1)
+        && validPageDb(p1)
+        && pageDbCorresponds(s1.m, p1)
+        && evalCode(smc_handler, s1, s2)
+        && AUCIdef() // XXX
+        ensures smchandlerInvariant(s1, s2)
+        ensures exists p2:PageDb :: smchandler(s1, p1, s2, p2)
+            && validPageDb(p2) && pageDbCorresponds(s2.m, p2)
+    {
+        var stack_bytes := KOM_STACK_SIZE() - BytesPerWord();
+        assert StackBytesRemaining(s1, stack_bytes);
+        reveal_sp_eval();
+        var block := sp_CCons(smc_handler, sp_CNil());
+        assert sp_eval(Block(block), s1, s2) by { assert evalBlock(block, s1, s2); }
+        var _, _, p2' := sp_lemma_smc_handler(block, s1, s2, stack_bytes, p1);
+        assert smchandler(s1, p1, s2, p2');
+        assert validPageDb(p2') && pageDbCorresponds(s2.m, p2');
+    }
+    
+    printAll();
 }
